\beginsection 3.

Use (3) to prove (2).
$$F_n={1\over\sqrt5}\left(\phi^n-\left(-{1\over\phi}\right)^n\right)\eqno(3)$$
$$\lim_{n\rightarrow\infty}{F_{n+1}\over F_n}=\phi\eqno(2)$$
\bigskip
We have
$$\eqalign{
{F_{n+1}\over F_n}&=
{
{1\over\sqrt5}\left(\phi^{n+1}-\left(-{1\over\phi}\right)^{n+1}\right)
\over
{1\over\sqrt5}\left(\phi^{n}-\left(-{1\over\phi}\right)^{n}\right)
}\cr
&=
{
\phi^{n+1}-\left(-{1\over\phi}\right)^{n+1}
\over
\phi^{n}-\left(-{1\over\phi}\right)^{n}
}\cr
&=
{\left(-{1\over\phi}\right)^{n}\over\left(-{1\over\phi}\right)^{n}}\times
{
\phi^{n+1}-\left(-{1\over\phi}\right)^{n+1}
\over
\phi^{n}-\left(-{1\over\phi}\right)^{n}
}\cr
&=
{
(-1)^n\phi-\left(-{1\over\phi}\right)^{2n+1}
\over
(-1)^n-\left(-{1\over\phi}\right)^{2n}
}\cr
}$$
Now evaluate the limit for $\phi>1$.
$$\eqalign{
\lim_{n\rightarrow\infty}{F_{n+1}\over F_n}&=
{
\phi\lim_{n\rightarrow\infty}(-1)^n-\lim_{n\rightarrow\infty}\left(-{1\over\phi}\right)^{2n+1}
\over
\lim_{n\rightarrow\infty}(-1)^n-\lim_{n\rightarrow\infty}\left(-{1\over\phi}\right)^{2n}
}\cr
&=
{
\phi\lim_{n\rightarrow\infty}(-1)^n-0
\over
\lim_{n\rightarrow\infty}(-1)^n-0
}\cr
&=\phi
}$$

\vfill
\eject

\beginsection 4.

Prove (3).
$$F_n={1\over\sqrt5}\left(\phi^n-\left(-{1\over\phi}\right)^n\right)\eqno(3)$$

\bigskip
Proof by induction.
For $n=0$ we have $F_0=0$ which is correct.
For $n=1$ we have
$$\eqalign{
F_1&={1\over\sqrt5}\left(\phi+{1\over\phi}\right)\cr
&={1\over\sqrt5}\left({\phi^2+1\over\phi}\right)\cr
&={1\over\sqrt5}\left({(10+2\sqrt5)/4\over(1+\sqrt5)/2}\right)\cr
&={(2\sqrt5+2)/4\over(1+\sqrt5)/2}\cr
&=1
}$$
which is also correct.
Now show that $F_{n}+F_{n+1}=F_{n+2}$.
$$\eqalign{
\sqrt5\,(F_n+F_{n+1})&=\phi^n-\left(-{1\over\phi}\right)^n
+\phi^{n+1}-\left(-{1\over\phi}\right)^{n+1}\cr
&=\phi^{n+2}\left(\phi^{-2}+\phi^{-1}\right)
-\left(-{1\over\phi}\right)^{n+2}
\left[
\left(-{1\over\phi}\right)^{-2}
+
\left(-{1\over\phi}\right)^{-1}
\right]\cr
&=
\phi^{n+2}\left(\phi^{-2}+\phi^{-1}\right)
-\left(-{1\over\phi}\right)^{n+2}
(\phi^2-\phi)\cr
&=\phi^{n+2}-\left(-{1\over\phi}\right)^{n+2}\cr
&=\sqrt5\,F_{n+2}
}$$
Hence by induction (3) is correct.

\vfill
\eject

\beginsection 5.

Use (1) to prove (4).
$$F_n=F_{n-1}+F_{n-2}\eqno(1)$$
$$\sum_{n=1}^\infty F_nt^n={t\over1-t-t^2}\eqno(4)$$
We have
$$\eqalign{
\sum_{n=1}^\infty F_nt^n&=F_0+F_1t+\sum_{n=2}^\infty(F_{n-1}+F_{n-2})t^n\cr
&=t+t\sum_{n=2}^\infty F_{n-1}t^{n-1}+t^2\sum_{n=2}^\infty F_{n-2}t^{n-2}\cr
&=t+t\sum_{n=1}^\infty F_nt^n+t^2\sum_{n=0}^\infty F_nt^n\cr
&=t+t\sum_{n=1}^\infty F_nt^n+t^2\sum_{n=1}^\infty F_nt^n+t^2F_0\cr
}$$
Now letting $X=\sum_{n=1}^\infty F_nt^n$ we have
$$X=t+tX+t^2X$$
Hence
$$X(1-t-t^2)=t$$
and finally
$$X={t\over1-t-t^2}$$

\end
