\beginsection 2. Using change-of-variable

From the inside cover of the book we have for uniform distributions
$$f(x)={1\over b-a},\qquad f(y)={1\over b-a}$$
hence
$$f(x,y)=f(x)f(y)={1\over(b-a)^2}$$
The Jacobian is already calculated, see Note 6 pages 33 and 34.
However, the hard part is transforming the limits of integration.
We have
$$(x,y)\rightarrow(x+y,x-y)$$
hence
$$\eqalign{
(a,a)&\rightarrow(2a,0)\cr
(b,b)&\rightarrow(2b,0)\cr
(a,b)&\rightarrow(a+b,a-b)\cr
(b,a)&\rightarrow(a+b,b-a)\cr
}$$
Follow along with the bottom of p. 34, except use $f(x,y)=1/(b-a)^2$ instead
of $f(x,y)=1$ and use $t$ instead of $y$...
$$f(t)={1\over2}\int_{2a+t}^{2b-t}{dt\over(b-a)^2}=-{t\over(b-a)^2}+{1\over b-a},
\qquad0\le t<b-a$$
$$f(t)={1\over2}\int_{2a-t}^{2b+t}{dt\over(b-a)^2}={t\over(b-a)^2}+{1\over b-a},
\qquad a-b\le t<0$$
and $f(t)=0$ everywhere else.

\end
