\beginsection Try out 4.3

Show that the function $t\mapsto c+r\tanh(t)$
is a strictly increasing function by
showing that its derivative is strictly positive.

\medskip\noindent
We have
$${d(\sinh t)\over dt}=\cosh t,\qquad{d(\cosh t)\over dt}=\sinh t$$
%We have
%$$\tanh t={e^t-e^{-t}\over e^t+e^{-t}}={e^t\over e^t+e^{-t}}-{e^{-t}\over e^t+e^{-t}}
%={1\over1+e^{-2t}}-{1\over e^{2t}+1}$$
Hence
$${d\tanh t\over dt}={d\left(\displaystyle{\sinh t\over\cosh t}\right)\over dt}
=(\cosh t)(\cosh t)^{-1}-(\sinh t)^2(\cosh t)^{-2}
=(\cosh t)^{-2}[(\cosh t)^2-(\sinh t)^2]={1\over (\cosh t)^2}$$

\end