\nopagenumbers
\noindent
For $s,t\in Q$ show that $s=t$ if and only if $s^*=t^*$.


\bigskip
\item{1.} Let $s=t$.

\item{2.} For all $r\in s^*$ we have $r<s$ by definition.
\item{3.} For $r<s$ we have $r<t$ by (1) hence $r\in t^*$.
\item{4.} Therefore $r\in s^*$ implies $r\in t^*$ hence $s^*\subseteq t^*$.

\item{5.} For all $r\in t^*$ we have $r<t$ by definition.
\item{6.} For $r<t$ we have $r<s$ by (1) hence $r\in s^*$.
\item{7.} Therefore $r\in t^*$ implies $r\in s^*$ hence $t^*\subseteq s^*$.

\item{8.} We have $s^*=t^*$ by (4) and (7).
\item{9.} Therefore $s=t$ implies $s^*=t^*$.

\item{10.} Let $s^*=t^*$.

\item{11.} Assume $s<t$.
\item{12.} We have $s\not\in s^*$ and $s\in t^*$, a contradiction of (10), hence $s\ge t$.
\item{13.} Assume $t<s$.
\item{14.} We have $t\in s^*$ and $t\not\in t^*$, a contradiction of (10), hence $t\ge s$.
\item{15.} We have $s=t$ by (12) and (14).
\item{16.} Therefore $s^*=t^*$ implies $s=t$.

\item{17.} Finally, by (9) and (16) we have  $s=t$ if and only if $s^*=t^*$.

% I like the way the contradictions in steps 10--16 turned out.
% In particular, the way $<$ leads to $\ge$ and then to equality.
% I can't think of a direct proof that is more compelling.

\end
