\parindent=0pt
Construct truth tables for the following logical expressions.

\bigskip
{\bf a.} $p\land(q\to p)$

$$\matrix{
p&q&q\to p&p\land(q\to p)\cr
T&T&T&T\cr
T&F&T&T\cr
F&T&F&F\cr
F&F&T&F\cr
}$$

\bigskip
{\bf b.} $(p\lor q)\to(p\land r)$

$$\matrix{
p&q&r&(p\lor q)&(p\land r)&(p\lor q)\to(p\land r)\cr
T&T&T&T&T&T\cr
T&T&F&T&F&F\cr
T&F&T&T&T&T\cr
T&F&F&T&F&F\cr
F&T&T&T&F&F\cr
F&T&F&T&F&F\cr
F&F&T&F&F&T\cr
F&F&F&F&F&T\cr
}$$

\bigskip
Determine if the following expressions are equivalent.

\bigskip
{\bf a.} $p\to(q\land r)$ and $(p\to q)\land r$.

$$\matrix{
p&q&r&q\land r&p\to(q\land r)\cr
T&T&T&T&T\cr
T&T&F&F&F\cr
T&F&T&F&F\cr
T&F&F&F&F\cr
F&T&T&T&T\cr
F&T&F&F&T\cr
F&F&T&F&T\cr
F&F&F&F&T\cr
}\qquad\qquad\matrix{
p&q&r&p\to q&(p\to q)\land r\cr
T&T&T&T&T\cr
T&T&F&T&T\cr
T&F&T&F&F\cr
T&F&F&F&F\cr
F&T&T&T&F\cr
F&T&F&T&F\cr
F&F&T&T&F\cr
F&F&F&T&F\cr
}$$
The truth tables show that the two expressions are not equivalent.

\bigskip
{\bf b.} $p\to(q\lor r)$ and $(p\to q)\lor(p\to r)$.

$$\matrix{
p&q&r&q\lor r&p\to(q\lor r)\cr
T&T&T&T&T\cr
T&T&F&T&T\cr
T&F&T&T&T\cr
T&F&F&F&F\cr
F&T&T&T&T\cr
F&T&F&T&T\cr
F&F&T&T&T\cr
F&F&F&F&T\cr
}\qquad\qquad\matrix{
p&q&r&p\to q&p\to r&(p\to q)\lor(p\to r)\cr
T&T&T&T&T&T\cr
T&T&F&T&F&T\cr
T&F&T&F&T&T\cr
T&F&F&F&F&F\cr
F&T&T&T&T&T\cr
F&T&F&T&T&T\cr
F&F&T&T&T&T\cr
F&F&F&T&T&T\cr
}$$
The truth tables show that the two expressions are indeed equivalent.

\vfill\eject
Negate the following expressions.

\bigskip
{\bf a.} $p\to(q\land{\sim}\,r)$
$$\eqalign{
{\sim}\,(p\to(q\land{\sim}\,r))&\equiv{\sim}\,({\sim}\,p\lor(q\land{\sim}\,r))\cr
&\equiv p\land{\sim}\,(q\land{\sim}\,r)\cr
&\equiv p\land({\sim}\,q\lor r)\cr
}$$

\bigskip
{\bf b.} ${\sim}\,p\to(q\lor r)$
$$\eqalign{
{\sim}\,({\sim}\,p\to(q\lor r))&\equiv{\sim}\,(p\lor(q\lor r))\cr
&\equiv{\sim}\,p\land{\sim}\,(q\lor r)\cr
&\equiv{\sim}\,p\land{\sim}\,q\land{\sim}\,r
}$$

\bigskip
{\bf c.} $p\land(q\to r)$
$$\eqalign{
{\sim}\,(p\land(q\to r))&\equiv{\sim}\,p\lor{\sim}\,({\sim}\,q\lor r)\cr
&\equiv{\sim}\,p\lor(q\land{\sim}\,r)\cr
}$$

\end

