\nopagenumbers
\parindent=0pt

{\bf Problem A.}

\bigskip
{\bf 1.} $gcd(180,252)=36$
$$\eqalign{
252\div180&=1\cdots72\cr
180\div72&=2\cdots36\cr
72\div36&=2
}$$

\bigskip
{\bf 2.} $gcd(513,187)=1$
$$\eqalign{
513\div187&=2\cdots139\cr
187\div139&=1\cdots48\cr
139\div48&=2\cdots43\cr
48\div43&=1\cdots5\cr
43\div5&=8\cdots3\cr
5\div3&=1\cdots2\cr
3\div2&=1\cdots1\cr
2\div1&=2\cr
}$$

\bigskip
{\bf 2.} $gcd(7655,1001)=1$
$$\eqalign{
7655\div1001&=7\cdots648\cr
1001\div648&=1\cdots353\cr
648\div353&=1\cdots295\cr
353\div295&=1\cdots58\cr
295\div58&=5\cdots5\cr
58\div5&=11\cdots3\cr
5\div3&=1\cdots2\cr
3\div2&=1\cdots1\cr
2\div1&=2\cr
}$$

\vfill
\eject

{\bf Problem B.}
$$\pmatrix{
1&0&\vdots&1030\cr
0&1&\vdots&521\cr
}$$
%
$R_1-R_2\rightarrow R_1$
$$\pmatrix{
1&-1&\vdots&509\cr
0&1&\vdots&521\cr
}$$
%
$R_2-R_1\rightarrow R_2$
$$\pmatrix{
1&-1&\vdots&509\cr
-1&2&\vdots&12\cr
}$$
%
$R_1-42R_2\rightarrow R_1$
$$\pmatrix{
43&-85&\vdots&5\cr
-1&2&\vdots&12\cr
}$$
%
$R_2-2R_1\rightarrow R_2$
$$\pmatrix{
43&-85&\vdots&5\cr
-87&172&\vdots&2\cr
}$$
%
$R_1-2R_2\rightarrow R_1$
$$\pmatrix{
217&-429&\vdots&1\cr
-87&172&\vdots&2\cr
}$$
%
We have $1|2$ therefore $gcd(1030,521)=1$.
In addition, reading off the top row we have
$x=217$ and $y=-429$.
Check that $1030x+521y=1$.
$$\eqalign
1030\cdot217+521\cdot(-429)=223{,}510-223{,}509=1$$

\vfill
\eject

{\bf Problem C.}
Show that if $a\in N$ and $b,c\in Z$ such that $b,c\ne0$ then
$gcd(ab,ac)=a\cdot gcd(b,c)$.
\bigskip
{\bf Proof.}
Let $a\in N$ and $b,c\in Z$ such that $b,c\ne0$.
Let $d=gcd(b,c)$ and $k\in Z$.
\medskip
(i) We want to show that $ad|ab$ and $ad|ac$.
By definition of GCD we have $d|b$ and $d|c$.
Then by Lemma 1.4 of Unit 9 and $N\subset Z$ we have
$ad|ab$ and $ad|ac$.
\medskip
(ii) Assume $k|ab$ and $k|ac$. We want to show that $k|ad$.
By the Euclidean Algorithm we have that there are $x,y\in Z$ such
that $d=bx+cy$, hence $ad=abx+acy$.
By Lemma 1.8 of Unit 9 we have $k|(abx+acy)$ for any $x,y\in Z$.
Hence $k|ad$.
\medskip
To summarize, we have $ad|ab$, $ad|ac$, and if $k\in Z$ such that
$k|ab$ and $k|ac$, then $k|ad$.
In addition, by $a\in N$ and closure we have $ad\in N$.
Therefore $ad=gcd(ab,ac)$.
Hence $a\cdot gcd(b,c)=gcd(ab,ac)$.

\end
