\nopagenumbers
\parindent=0pt

{\bf Problem A.}
Let $f(x),g(x)\in F[x]$ such that $f(x)\ne0$.
If $f(x)\,|\,g(x)$ then $f(x)\,|\,[g(x)+(2x-1)f(x)]$.

\medskip

{\bf Proof.}
Let $f(x),g(x)\in F[x]$ such that $f(x)\ne0$.
Assume $f(x)\,|\,g(x)$.
Then there is a $t(x)\in F[x]$ such that $t(x)f(x)=g(x)$.
Hence
$$g(x)+(2x-1)f(x)=t(x)f(x)+(2x-1)f(x)=(t(x)+2x-1)f(x)$$
Therefore $f(x)\,|\,[g(x)+(2x-1)f(x)]$.

\bigskip
\bigskip

{\bf Problem B.}
Let $f(x),g(x),h(x)\in F[x]$ such that $f(x)\ne0$.
If $f(x)\,|\,g(x)$ and $f(x)\,|\,h(x)$ then
$$f(x)\,|\,[(2x+1)g(x)-(3x^6-x^3+1)h(x)]$$

\medskip

{\bf Proof.}
Let $f(x),g(x),h(x)\in F[x]$ such that $f(x)\ne0$.
Assume $f(x)\,|\,g(x)$ and $f(x)\,|\,h(x)$.
Then there are $s(x),t(x)\in F[x]$ such that
$s(x)f(x)=g(x)$ and $t(x)f(x)=h(x)$.
Hence
$$\eqalign{(2x+1)g(x)-(3x^6-x^3+1)h(x)
&=(2x+1)s(x)f(x)-(3x^6-x^3+1)t(x)f(x)\cr
&=[(2x+1)s(x)-(3x^6-x^3+1)t(x)]f(x)}$$
Hence $f(x)\,|\,[(2x+1)g(x)-(3x^6-x^3+1)h(x)]$.

\bigskip
\bigskip

{\bf Problem C.}
Let $f(x)\in F[x]$ such that $f(x)\ne0$.
If $f(x)\,|\,122$ then $\deg(f(x))=0$.

\medskip

{\bf Proof.}
Let $f(x)\in F[x]$ such that $f(x)\ne0$.
Assume $f(x)\,|\,122$.
Then there is a $t(x)\in F[x]$ such that $f(x)t(x)=122$.
Hence
$\deg(f\cdot t)=\deg(122)=0$.
Therefore
$$\deg(f)+\deg(t)=0$$
Note that $t(x)\ne0$.
Since $f(x),t(x)\ne0$ we have $\deg(f),\deg(t)\in\{0,N\}$.
Therefore the only solution is $\deg(f)=\deg(t)=0$.
Hence $\deg(f)=0$.

\end
