\parindent=0pt
\nopagenumbers

April 4, 2003. Exercise from A=B, p. 50.

$$\sum_k
\bigg({n\atop k}\bigg)
\bigg({n+a\atop k}\bigg)
\bigg({n-a\atop n-k}\bigg)
$$

We have...

$$
t_k=
\bigg({n\atop k}\bigg)
\bigg({n+a\atop k}\bigg)
\bigg({n-a\atop n-k}\bigg)
$$
and
$$
t_{k+1}=
\bigg({n\atop k+1}\bigg)
\bigg({n+a\atop k+1}\bigg)
\bigg({n-a\atop n-k-1}\bigg)
$$

Compute $t_{k+1}/t_k$ by combining 1st, 2nd and 3rd terms.

$${
\displaystyle{\left({n\atop k+1}\right)}
\over
\displaystyle{\left({n\atop k}\right)}
}=
{
n!/[(n-k-1)!(k+1)!]
\over
n!/[(n-k)!k!]
}
=
{(n-k)!k!\over(n-k-1)!(k+1)!}
=
{(n-k)\over(k+1)}
$$

$${
\displaystyle{\left({n+a\atop k+1}\right)}
\over
\displaystyle{\left({n+a\atop k}\right)}
}=
{
(n+a)!/[(n+a-k-1)!(k+1)!]
\over
(n+a)!/[(n+a-k)!k!]
}
=
{(n+a-k)!k!\over(n+a-k-1)!(k+1)!}
=
{(n+a-k)\over(k+1)}
$$

$${
\displaystyle{\left({n-a\atop n-k-1}\right)}
\over
\displaystyle{\left({n-a\atop n-k}\right)}
}=
{
(n-a)!/[(k-a+1)!(n-k-1)!]
\over
(n-a)!/[(k-a)!(n-k)!]
}
=
{(k-a)!(n-k)!\over(k-a+1)!(n-k-1)!}
=
{(n-k)\over(k-a+1)}
$$

$$\eqalign{
{t_{k+1}\over t_k}
&=
{(n-k)\over(k+1)}
\times
{(n+a-k)\over(k+1)}
\times
{(n-k)\over(k-a+1)}\cr
&=
-1\times
{(k-n)\over(k+1)}
\times
{(k-n-a)\over(k+1)}
\times
{(k-n)\over(k-a+1)}\cr
&=
{}_3F_2\left[
\matrix{
-n&-n&-n-a\cr
1&-a+1&{}};\;-1\right]
}$$

\end
