\beginsection{Mandl and Shaw Problem 3.2}

From Eq.~3.27 we have
$$\eqalign{
\phi(x)&=
\sum_{\bf k}\left(1\over2V\omega({\bf k})\right)^{1/2}
[a({\bf k})\exp(-ikx)+b^\dagger({\bf k})\exp(ikx)]\cr
\phi^\dagger(x)&=
\sum_{\bf k}\left(1\over2V\omega({\bf k})\right)^{1/2}
[b({\bf k})\exp(-ikx)+a^\dagger({\bf k})\exp(ikx)]\cr
}$$
From Eq.~3.36 we have
$$\eqalign{
\phi(x)&={1\over\sqrt2}(\phi_1(x)+i\phi_2(x))\cr
\phi^\dagger(x)&={1\over\sqrt2}(\phi_1(x)-i\phi_2(x))\cr
}$$
Now, given
$$\eqalign{
\phi_1(x)&=\sum_{\bf k}\left(1\over2V\omega({\bf k})\right)^{1/2}
[a_1({\bf k})\exp(-ikx)+a_1^\dagger({\bf k})\exp(ikx)] \cr
\phi_2(x)&=\sum_{\bf k}\left(1\over2V\omega({\bf k})\right)^{1/2}
[a_2({\bf k})\exp(-ikx)+a_2^\dagger({\bf k})\exp(ikx)] \cr
}$$
show that
$$\eqalign{
a({\bf k})&={1\over\sqrt2}[a_1({\bf k})+ia_2({\bf k})]\cr
b({\bf k})&={1\over\sqrt2}[a_1({\bf k})-ia_2({\bf k})]\cr
}$$

\beginsection{Solution}

This problem seems simple compared to the epic Problem 3.1.
All we have to do is take the Fourier transform of $\phi$,
$\phi^\dagger$, $\phi_1$ and $\phi_2$.
%
$$\eqalign{
\int_{-\infty}^{+\infty}\phi(x)\exp(ikx)\,dx&=
\left(1\over2V\omega({\bf k})\right)^{1/2}
a({\bf k})\cr
\int_{-\infty}^{+\infty}\phi^\dagger(x)\exp(ikx)\,dx&=
\left(1\over2V\omega({\bf k})\right)^{1/2}
b({\bf k})\cr
\int_{-\infty}^{+\infty}\phi_1(x)\exp(ikx)\,dx&=
\left(1\over2V\omega({\bf k})\right)^{1/2}
a_1({\bf k})\cr
\int_{-\infty}^{+\infty}\phi_2(x)\exp(ikx)\,dx&=
\left(1\over2V\omega({\bf k})\right)^{1/2}
a_2({\bf k})\cr
}$$

\vfill
\break

{\tt\obeylines
clear()
N = 2
V = L\char94 3
x = (x0,x1,x2,x3)
k() = (omega(), 2 pi / L n1, 2 pi / L n2, 2 pi / L n3)
omega() = sqrt(m\char94 2 + (2 pi / L (n1,n2,n3))\char94 2)
phi = sum(n1, -N, N, sum(n2, -N, N, sum(n3, -N, N,
\ (a(n1,n2,n3) exp(-i dot(k(),x)) + b(n1,n2,n3) exp(i dot(k(),x))) /
\ sqrt(2 V omega())
)))
phi1 = sum(n1, -N, N, sum(n2, -N, N, sum(n3, -N, N,
\ (a1(n1,n2,n3) exp(-i dot(k(),x)) + a1dag(n1,n2,n3) exp(i dot(k(),x))) /
\ sqrt(2 V omega())
)))
phi2 = sum(n1, -N, N, sum(n2, -N, N, sum(n3, -N, N,
\ (a2(n1,n2,n3) exp(-i dot(k(),x)) + a2dag(n1,n2,n3) exp(i dot(k(),x))) /
\ sqrt(2 V omega())
)))
n1 = 1
n2 = 2
n3 = -1
A = (phi1 + i phi2) / sqrt(2)
A = A V exp(i dot(k(),x))
A = filter(A,x0,x1,x2,x3)
display(A)
B = phi V exp(i dot(k(),x))
B = filter(B,x0,x1,x2,x3)
display(B)
T = (a1(n1,n2,n3) + i a2(n1,n2,n3)) / sqrt(2)
B = eval(subst(T,a(n1,n2,n3),B))
A - B
}

